wip

theories/examples/copy_word.v
@@ -179,32 +179,38 @@ Section copy_word.
     bne_I R7
     ].
 
-  Definition cycle prog step base := c_pre step base ++ (prog step) ++ c_post.
+  Definition c_loop prog := prog ++ c_post.
+  Definition cycle prog step base := c_pre step base ++ c_loop prog.
 
-  Lemma c_loop {progpage sacc i q} {base : Imm} {n : nat} (body : list Word) step prog (P : Word -> iProp Σ) :
+
+  Lemma c_loop_spec {progpage sacc i q} {base : Imm} {n : nat} (body : list Word) step prog (P : Word -> iProp Σ) :
     of_imm base = ((of_pid progpage) ^+ 3)%f ->
     S n = Z.to_nat (finz.to_z (of_imm step)) ->
     progpage ∈ sacc ->
     seq_in_page (of_pid progpage) (length (cycle prog step base)) progpage ->
     (forall l step, length (cycle prog l base) = length (cycle prog step base)) ->
-    (∀ v (v' : Word) v'' (step : Imm), ⌜v = Z.to_nat (finz.to_z v') ∧ (v <= S n)⌝ -∗ {PAR{{ (P (v' ^+ 1)%f) ∗ PC @@ i ->r ((of_pid progpage) ^+ 3)%f
-                         ∗ R6 @@ i ->r v''
-                         ∗ R5 @@ i ->r step
-                         ∗ R7 @@ i ->r ((of_pid progpage) ^+ 3)%f
+    (∀ v (v' : Word) progaddr,
+      ⌜ v = Z.to_nat (finz.to_z v') ⌝ -∗
+      ⌜ v <= S n ⌝-∗
+      ⌜ seq_in_page progaddr (length prog) progpage ⌝ -∗
+    {PAR{{ (P (v' ^+ 1)%f) ∗ PC @@ i ->r progaddr
+                         ∗ R6 @@ i ->r I0
+                         ∗ R5 @@ i ->r (v' ^+ 1)%f
+                         ∗ R7 @@ i ->r progaddr
                          ∗ (∃ r, R8 @@ i ->r r)
                          ∗ (∃ nz, NZ @@ i ->r nz)             
                          ∗ A@i :={q}[sacc]
-                         ∗ (program' (cycle prog step base) (of_pid progpage))
+                         ∗ (program' prog progaddr)
             }}} ExecI @ i
-    {{{ RET ExecI; (P v') ∗ PC @@ i ->r (((of_pid progpage) ^+ 3)%f ^+ (length (prog step)))%f
-                         ∗ R6 @@ i ->r v''
-                         ∗ R5 @@ i ->r step
-                         ∗ R7 @@ i ->r ((of_pid progpage) ^+ 3)%f
+    {{{ RET ExecI; (P v') ∗ PC @@ i ->r (progaddr ^+ (length prog))%f
+                         ∗ R6 @@ i ->r I0
+                         ∗ R5 @@ i ->r (v' ^+ 1)%f
+                         ∗ R7 @@ i ->r progaddr
                          ∗ (∃ r, R8 @@ i ->r r)
                          ∗ (∃ nz, NZ @@ i ->r nz)  
                          ∗ A@i :={q}[sacc]
-                         ∗ (program' (cycle prog step base) (of_pid progpage))
-    }}}%I)
+                         ∗ (program' prog progaddr)
+    }}}%I)%I
     ⊢  {PAR{{ (P step) ∗ PC @@ i ->r (of_pid progpage)
                        ∗ (∃ r5, R5 @@ i ->r r5)
                        ∗ (∃ r6, R6 @@ i ->r r6)
@@ -225,13 +231,12 @@ Section copy_word.
     }}}%I.
   Proof.
     iIntros (Hbase Hn Hprpain Hseq Hlen) "#Htriple".
-    iInduction n as [| n] "IH" forall (step Hn Hseq Hlen).
-    - rename Hn into eq.
+    rename Hn into eq.
       rename Hseq into c.
       apply seq_in_page_forall in c.
       iIntros (Φ).
       iModIntro.
-      iIntros "(HPstep & Hpc & [% Hr5] & [% Hr6] & [% Hr7] & [% Hr8] &[% Hnz] & Hacc & Hprog) HΦ".
+      iIntros "(HPstep & Hpc & [% Hr5] & [% Hr6] & [% Hr7] & Hr8 & Hnz & Hacc & Hprog) HΦ".
       rewrite <-parwp_sswp.
       iDestruct "Hprog" as "(p_start & Hprog)". 
       iDestruct ((mov_word (of_pid progpage) step R5) with "[Hpc Hacc Hr5 p_start]") as "J".
@@ -265,50 +270,106 @@ Section copy_word.
       iApply "J".
       iModIntro.
       iIntros "(Hpc & Hinstr3 & Hacc & Hr7)".
-      iDestruct ("Htriple" $! 0 I0 I0 step _ with "") as "#HprogSpec".
-      Unshelve.
-      2 : {
-        split.
-        rewrite /I0.
-        simpl.
-        lia.
-        solve_finz.
-      }
-      iSpecialize ("HprogSpec" $! (fun k => (⌜k = ExecI⌝
-                                     ∗ P I0
-                                            ∗ PC @@ i ->r ((progpage ^+ 3) ^+ length (prog step))%f
-                                            ∗ R5 @@ i ->r step
-                                            ∗ R6 @@ i ->r I0
-                                            ∗ R7 @@ i ->r (progpage ^+ 3)%f
-                                            ∗ (∃ r : handle, R8 @@ i ->r r)
-                                            ∗ (∃ nz, NZ @@ i ->r nz)             
-                                            ∗ A@i:={q}[sacc]
-                                            ∗ program' (cycle prog step base) progpage)%I) with "").
-      iDestruct ("HprogSpec" with "[HPstep Hpc Hr5 Hr6 Hr7 Hr8 Hnz Hacc Hprog Hinstr1 Hinstr2 Hinstr3]") as "J".
+     Admitted.
+
+
+  Lemma c_loop_ind_spec {progaddr progpage sacc i q} {base : Imm} {n : nat} (body : list Word) step prog (P : Word -> iProp Σ) :
+    of_imm base = (progaddr)%f ->
+    S n = Z.to_nat (finz.to_z (of_imm step)) ->
+    addr_in_page progaddr progpage ->
+    progpage∈ sacc ->
+    seq_in_page progaddr (length (c_loop prog)) progpage ->
+    (∀ v (v' : Word) ,
+      ⌜ v = Z.to_nat (finz.to_z v') ⌝ -∗
+      ⌜ v <= S n ⌝-∗
+      ⌜ seq_in_page progaddr (length prog) progpage ⌝ -∗
+    {PAR{{ (P (v' ^+ 1)%f) ∗ PC @@ i ->r progaddr
+                         ∗ R6 @@ i ->r I0
+                         ∗ R5 @@ i ->r (v' ^+ 1)%f
+                         ∗ R7 @@ i ->r progaddr
+                         ∗ (∃ r, R8 @@ i ->r r)
+                         ∗ (∃ nz, NZ @@ i ->r nz)
+                         ∗ A@i :={q}[sacc]
+                         ∗ (program' prog progaddr)
+            }}} ExecI @ i
+    {{{ RET ExecI; (P v') ∗ PC @@ i ->r (progaddr ^+ (length prog))%f
+                         ∗ R6 @@ i ->r I0
+                         ∗ R5 @@ i ->r (v' ^+ 1)%f
+                         ∗ R7 @@ i ->r progaddr
+                         ∗ (∃ r, R8 @@ i ->r r)
+                         ∗ (∃ nz, NZ @@ i ->r nz)
+                         ∗ A@i :={q}[sacc]
+                         ∗ (program' prog progaddr)
+    }}}%I)%I
+    ⊢  {PAR{{ (P step) ∗ PC @@ i ->r progaddr
+                       ∗ R5 @@ i ->r step
+                       ∗ R6 @@ i ->r I0
+                       ∗ R7 @@ i ->r progaddr
+                       ∗ (∃ r8, R8 @@ i ->r r8)
+                       ∗ (∃ nz, NZ @@ i ->r nz)
+                       ∗ A@i :={q}[sacc]
+                       ∗ program' (c_loop prog) progaddr
+       }}} ExecI @ i
+    {{{ RET ExecI; (P I0) ∗ PC @@ i ->r (progaddr ^+ (length (c_loop prog )))%f
+                          ∗ R5 @@ i ->r (step ^- (S n))%f
+                          ∗ R6 @@ i ->r I0
+                          ∗ R7 @@ i ->r progaddr
+                          ∗ R8 @@ i ->r I1
+                          ∗ (∃ nz, NZ @@ i ->r nz)
+                          ∗ A@i :={q}[sacc]
+                          ∗ program' (c_loop prog) progaddr
+    }}}%I.
+     Proof.
+    iIntros (Hbase Hn Hprogaddrin Hprpain Hseq ) "#Htriple".
+    rename Hn into eq.
+      rename Hseq into c.
+      (* apply seq_in_page_forall in c. *)
+      iIntros (Φ).
+      iModIntro.
+      iIntros "(HPstep & Hpc & Hr5 & Hr6 & Hr7 & Hr8 & Hnz & Hacc & Hprog) HΦ".
+    iInduction n as [| n] "IH" forall (step eq c).
+      - iDestruct ("Htriple" $! 0 I0 with "") as "#HprogSpec".
+      iSpecialize ("HprogSpec"   with "[//] [] []").
+      iPureIntro;lia.
+      { admit.  }
+        assert (Htemp : (finz.seq progaddr (length prog)  ++ finz.seq (progaddr ^+ (length prog))%f 4) = finz.seq progaddr (length (prog ++ c_post))).
+        { rewrite app_length.
+          assert (length c_post = 4) as ->.
+          done.
+          rewrite (finz_seq_decomposition ((length prog) + 4) progaddr (length prog)).
+          rewrite minus_plus.
+          reflexivity.
+          lia.
+        }
+        rewrite /program' /c_loop .
+        rewrite -Htemp.
+        iDestruct (big_sepL2_app_inv with "Hprog") as "(Hprog & Hcpost)".
+        { rewrite finz_seq_length.  left;done. }
+      iDestruct ("HprogSpec" with "[HPstep Hpc Hr5 Hr6 Hr7 Hr8 Hnz Hacc Hprog ]") as "J".
       iFrame.
-      rewrite Hbase.
-      assert (Hn : (progpage ^+ 3)%f = (((progpage ^+ 1) ^+ 1) ^+ 1)%f).
-      solve_finz.
-      rewrite Hn.
-      clear Hn.
-      iFrame.
-      assert (Htemp : (I0 ^+ 1)%f = step).
+      assert ( (I0 ^+ 1)%f = step) as ->.
       rewrite /I0 //.
       simpl.
       apply finz_to_z_eq.
       simpl.
       lia.
-      rewrite Htemp. clear Htemp.
-      iFrame.
-      iSplitL "Hr8".
-      iExists r8.
-      iFrame.
-      iExists nz.
       iFrame.
       iApply parwp_parwp.
       iApply (parwp_strong_mono with "[J]").
       instantiate (1 := ⊤).
       set_solver.
+      instantiate (3:=
+      (fun k => (⌜k = ExecI⌝
+                                     ∗ P I0
+                                            ∗ PC @@ i ->r (progaddr ^+ (length prog))%f
+                                            ∗ R5 @@ i ->r (I0 ^+ 1)%f
+                                            ∗ R6 @@ i ->r I0
+                                            ∗ R7 @@ i ->r progaddr
+                                            ∗ (∃ r : handle, R8 @@ i ->r r)
+                                            ∗ (∃ nz, NZ @@ i ->r nz)
+                                            ∗ A@i:={q}[sacc]
+                                            ∗ program' prog  progaddr )%I)
+      ).
       iApply "J".
       iModIntro.
       iIntros "(? & ? & ? & ? & ? & ? & ? & ? & ?)".
@@ -317,79 +378,82 @@ Section copy_word.
       iIntros (k) "(%Heq & HP & Hpc & Hr5 & Hr6 & Hr7 & [%r8' Hr8] & [%nz' Hnz] & Hacc & Hprog)".
       subst k.
       iModIntro.
-      assert (Hn : cycle prog step base = (c_pre step base ++ (prog step)) ++ c_post).
-      auto.
-      rewrite /program'.
-      assert (Hn' : finz.seq progpage (length (cycle prog step base)) = (finz.seq progpage 3 ++ finz.seq (progpage ^+ 3)%f (length (prog step))) ++ finz.seq ((progpage ^+ 3) ^+ (length (prog step)))%f 4).
-      {
-        assert (Htemp : (finz.seq progpage 3 ++ finz.seq (progpage ^+ 3)%f (length (prog step) + 3 - 3)) = finz.seq progpage (length (prog step) + 3)).
-        {
-          rewrite (finz_seq_decomposition ((length (prog step)) + 3) progpage 3).
-          reflexivity.
-          lia.
-        }
-        assert (Htemp' : length (prog step) = (length (prog step) + 3 - 3)).
-        lia.
-        rewrite <-Htemp' in Htemp.
-        clear Htemp'.
-        rewrite Htemp.
-        clear Htemp.
-        assert (Htemp : (finz.seq progpage (length (prog step) + 3) ++ finz.seq ((progpage ^+ 3) ^+ length (prog step))%f 4) = finz.seq progpage (length (cycle prog step base))).
-        {
-          rewrite (finz_seq_decomposition (length (cycle prog step base)) progpage (length (prog step) + 3)).
-          f_equal.
-          assert (Htemp' : ((progpage ^+ 3) ^+ length (prog step))%f = (progpage ^+ (length (prog step) + 3)%nat)%f).
-          solve_finz.
-          rewrite Htemp'.
-          clear Htemp'.
-          assert (Htemp' : (length (cycle prog step base) - (length (prog step) + 3)) = 4).
-          rewrite /cycle.
-          simpl.
-          rewrite Nat.add_comm.
-          simpl.
-          rewrite app_length.
-          rewrite minus_plus.
-          rewrite /c_post.
-          reflexivity.
-          rewrite Htemp'.
-          clear Htemp'.
-          reflexivity.
-          rewrite /cycle.
-          do 2 (rewrite app_length).
-          rewrite PeanoNat.Nat.add_assoc.          
-          rewrite (Nat.add_comm (length (c_pre step base))).
-          rewrite <-PeanoNat.Nat.add_assoc.
-          apply plus_le_compat_l.
-          simpl.
-          lia.
-        }
-        rewrite <-Htemp.
-        clear Htemp.
-        reflexivity.
-      }
-      rewrite Hn'.
-      rewrite /cycle.
-      rewrite (app_assoc (c_pre step base)).
-      iDestruct (big_sepL2_app_inv with "Hprog") as "(Uold & U)".
-      simpl.
-      by right.      
-      iDestruct "U" as "(p_start & U)".
-      iDestruct ((mov_word ((progpage ^+ 3) ^+ length (prog step))%f I1 R8) with "[Hpc Hacc Hr8 p_start]") as "J".
-      3 : { rewrite ->Forall_forall in c. apply c. rewrite /cycle. rewrite elem_of_list_In. rewrite (app_assoc (c_pre step base)). do 2 (rewrite app_length).  simpl.
-            do 3 right.
-            assert (Htemp : (((progpage ^+ 1) ^+ 1) ^+ 1)%f = (progpage ^+ 3)%f).
-            solve_finz.
-            rewrite Htemp.
-            clear Htemp.
-            rewrite (finz_seq_decomposition (length (prog step) + 4) (progpage ^+ 3)%f (length (prog step))); [|lia].           
+      (* assert (Hn : cycle prog step base = (c_pre step base ++ (prog step)) ++ c_post). *)
+      (* auto. *)
+      (* rewrite /program'. *)
+      (* assert (Hn' : finz.seq progpage (length (cycle prog step base)) = (finz.seq progpage 3 ++ finz.seq (progpage ^+ 3)%f (length (prog step))) ++ finz.seq ((progpage ^+ 3) ^+ (length (prog step)))%f 4). *)
+      (* { *)
+      (*   assert (Htemp : (finz.seq progpage 3 ++ finz.seq (progpage ^+ 3)%f (length (prog step) + 3 - 3)) = finz.seq progpage (length (prog step) + 3)). *)
+      (*   { *)
+      (*     rewrite (finz_seq_decomposition ((length (prog step)) + 3) progpage 3). *)
+      (*     reflexivity. *)
+      (*     lia. *)
+      (*   } *)
+      (*   assert (Htemp' : length (prog step) = (length (prog step) + 3 - 3)). *)
+      (*   lia. *)
+      (*   rewrite <-Htemp' in Htemp. *)
+      (*   clear Htemp'. *)
+      (*   rewrite Htemp. *)
+      (*   clear Htemp. *)
+      (*   assert (Htemp : (finz.seq progpage (length (prog step) + 3) ++ finz.seq ((progpage ^+ 3) ^+ length (prog step))%f 4) = finz.seq progpage (length (cycle prog step base))). *)
+      (*   { *)
+      (*     rewrite (finz_seq_decomposition (length (cycle prog step base)) progpage (length (prog step) + 3)). *)
+      (*     f_equal. *)
+      (*     assert (Htemp' : ((progpage ^+ 3) ^+ length (prog step))%f = (progpage ^+ (length (prog step) + 3)%nat)%f). *)
+      (*     solve_finz. *)
+      (*     rewrite Htemp'. *)
+      (*     clear Htemp'. *)
+      (*     assert (Htemp' : (length (cycle prog step base) - (length (prog step) + 3)) = 4). *)
+      (*     rewrite /cycle. *)
+      (*     simpl. *)
+      (*     rewrite Nat.add_comm. *)
+      (*     simpl. *)
+      (*     rewrite app_length. *)
+      (*     rewrite minus_plus. *)
+      (*     rewrite /c_post. *)
+      (*     reflexivity. *)
+      (*     rewrite Htemp'. *)
+      (*     clear Htemp'. *)
+      (*     reflexivity. *)
+      (*     rewrite /cycle. *)
+      (*     do 2 (rewrite app_length). *)
+      (*     rewrite PeanoNat.Nat.add_assoc.           *)
+      (*     rewrite (Nat.add_comm (length (c_pre step base))). *)
+      (*     rewrite <-PeanoNat.Nat.add_assoc. *)
+      (*     apply plus_le_compat_l. *)
+      (*     simpl. *)
+      (*     lia. *)
+      (*   } *)
+      (*   rewrite <-Htemp. *)
+      (*   clear Htemp. *)
+      (*   reflexivity. *)
+      (* } *)
+      (* rewrite Hn'. *)
+      (* rewrite /cycle. *)
+      (* rewrite (app_assoc (c_pre step base)). *)
+      (* iDestruct (big_sepL2_app_inv with "Hprog") as "(Uold & U)". *)
+      (* simpl. *)
+      (* by right.       *)
+      pose proof c as Hseq.
+      apply seq_in_page_forall in c.
+      iDestruct "Hcpost" as "(p_start & Hcpost)".
+      iDestruct ((mov_word (progaddr ^+ length prog )%f I1 R8) with "[Hpc Hacc Hr8 p_start]") as "J".
+      5: { iFrame. }
+      3 : { instantiate (1:= progpage). rewrite ->Forall_forall in c. apply c. rewrite /c_loop. rewrite elem_of_list_In.
+            rewrite -Htemp.
+            (* do 2 right. *)
+            (* assert (Htemp : (((progpage ^+ 1) ^+ 1) ^+ 1)%f = (progpage ^+ 3)%f). *)
+            (* solve_finz. *)
+            (* rewrite Htemp. *)
+            (* clear Htemp. *)
+
+            (* rewrite (finz_seq_decomposition (length (prog step) + 4) (length prog)); [|lia]. *)
             apply in_or_app.
             right.
             rewrite <-elem_of_list_In.
-            rewrite minus_plus.
             set_solver.
       }
       3 : { apply Hprpain. }
-      3 : { iFrame. }
       auto.
       by rewrite decode_encode_instruction.
       iApply parwp_sswp.
@@ -397,42 +461,38 @@ Section copy_word.
       iModIntro.
       iIntros "(Hpc & Hinstr4 & Hacc & Hr8)".
       iApply parwp_sswp.
-      iDestruct "U" as "(p_start & U)".
-      iDestruct ((sub (((progpage ^+ 3) ^+ length (prog step)) ^+ 1)%f R5 R8) with "[Hpc Hacc Hr5 Hr8 p_start]") as "J".
-      3 : { rewrite ->Forall_forall in c. apply c. rewrite /cycle. rewrite elem_of_list_In. rewrite (app_assoc (c_pre step base)). do 2 (rewrite app_length).  simpl.
-            do 3 right.
-            assert (Htemp : (((progpage ^+ 1) ^+ 1) ^+ 1)%f = (progpage ^+ 3)%f).
-            solve_finz.
-            rewrite Htemp.
-            clear Htemp.
-            rewrite (finz_seq_decomposition (length (prog step) + 4) (progpage ^+ 3)%f (length (prog step))); [|lia].           
+      iDestruct "Hcpost" as "(p_start & Hcpost)".
+      iDestruct ((sub ((progaddr ^+ length prog ) ^+ 1)%f R5 R8) with "[Hpc Hacc Hr5 Hr8 p_start]") as "J".
+      5: { iFrame. }
+      3 : { instantiate (1:= progpage). rewrite ->Forall_forall in c. apply c. rewrite /c_loop. rewrite elem_of_list_In.
+            rewrite -Htemp.
+            (* do 2 right. *)
+            (* assert (Htemp : (((progpage ^+ 1) ^+ 1) ^+ 1)%f = (progpage ^+ 3)%f). *)
+            (* solve_finz. *)
+            (* rewrite Htemp. *)
+            (* clear Htemp. *)
+
+            (* rewrite (finz_seq_decomposition (length (prog step) + 4) (length prog)); [|lia]. *)
             apply in_or_app.
             right.
             rewrite <-elem_of_list_In.
-            rewrite minus_plus.
             set_solver.
       }
       3 : { apply Hprpain. }
-      3 : { iFrame. }
       auto.
       by rewrite decode_encode_instruction.
       iApply "J".
       iModIntro.
       iIntros "(Hpc & Hinstr5 & Hr5 & Hr8 & Hacc)".
       iApply parwp_sswp.
-      iDestruct "U" as "(p_start & U)".
-      iDestruct ((cmp_reg ((((progpage ^+ 3) ^+ length (prog step)) ^+ 1) ^+ 1)%f R6 R5) with "[Hpc Hacc Hr5 Hr6 Hnz p_start]") as "J".
-      3 : { rewrite ->Forall_forall in c. apply c. rewrite /cycle. rewrite elem_of_list_In. rewrite (app_assoc (c_pre step base)). do 2 (rewrite app_length).  simpl.
-            do 3 right.
-            assert (Htemp : (((progpage ^+ 1) ^+ 1) ^+ 1)%f = (progpage ^+ 3)%f).
-            solve_finz.
-            rewrite Htemp.
-            clear Htemp.
-            rewrite (finz_seq_decomposition (length (prog step) + 4) (progpage ^+ 3)%f (length (prog step))); [|lia].           
+      iDestruct "Hcpost" as "(p_start & Hcpost)".
+      iDestruct ((cmp_reg (((progaddr ^+ length prog ) ^+ 1) ^+ 1)%f R6 R5) with "[Hpc Hacc Hr5 Hr6 Hnz p_start]") as "J".
+      5: {iFrame. }
+      3 : { instantiate (1:= progpage). rewrite ->Forall_forall in c. apply c. rewrite /c_loop. rewrite elem_of_list_In.
+            rewrite -Htemp.
             apply in_or_app.
             right.
             rewrite <-elem_of_list_In.
-            rewrite minus_plus.
             set_solver.
       }
       reflexivity.
@@ -442,46 +502,32 @@ Section copy_word.
       iApply "J".
       iModIntro.
       iIntros "(Hpc & Hinstr6 & Hr6 & Hr5 & Hacc & Hnz)".
-      assert (Htemp : (I0 <? step ^- I1)%f = false).
+      assert ((I0 <? I0 ^+ 1 ^- I1)%f = false) as ->.
       {
-        assert ((step ^- I1)%f = I0) as ->.
-        rewrite /I0.
+        rewrite /I0 /I1.
         simpl.
         solve_finz.
-        solve_finz.     
       }
-      rewrite Htemp.
-      clear Htemp.
-      assert (Htemp : (step ^- I1 <? I0)%f = false).
+      assert ((I0 ^+ 1 ^- I1 <? I0)%f = false) as ->.
       {
-        assert ((step ^- I1)%f = I0) as ->.
-        rewrite /I0.
+        rewrite /I0 /I1.
         simpl.
         solve_finz.
-        solve_finz.
       }
-      rewrite Htemp.
-      clear Htemp.
       iApply parwp_sswp.
-      iDestruct "U" as "(p_start & U)".      
-      iDestruct ((bne (((((progpage ^+ 3) ^+ length (prog step)) ^+ 1) ^+ 1) ^+ 1)%f R7) with "[Hpc Hacc Hr7 Hnz p_start]") as "J".
-      3 : { rewrite ->Forall_forall in c. apply c. rewrite /cycle. rewrite elem_of_list_In. rewrite (app_assoc (c_pre step base)). do 2 (rewrite app_length). simpl.
-            do 3 right.
-            assert (Htemp : (((progpage ^+ 1) ^+ 1) ^+ 1)%f = (progpage ^+ 3)%f).
-            solve_finz.
-            rewrite Htemp.
-            clear Htemp.
-            rewrite (finz_seq_decomposition (length (prog step) + 4) (progpage ^+ 3)%f (length (prog step))); [|lia].           
+      iDestruct "Hcpost" as "(p_start & Hcpost)".
+      iDestruct ((bne ((((progaddr ^+ length prog ) ^+ 1) ^+ 1) ^+ 1)%f R7) with "[Hpc Hacc Hr7 Hnz p_start]") as "J".
+      5 : { iFrame. }
+      3 : { instantiate (1:= progpage). rewrite ->Forall_forall in c. apply c. rewrite /c_loop. rewrite elem_of_list_In.
+            rewrite -Htemp.
             apply in_or_app.
             right.
             rewrite <-elem_of_list_In.
-            rewrite minus_plus.
             set_solver.
       }
       reflexivity.
       apply decode_encode_instruction.
       apply Hprpain.
-      iFrame.
       iApply "J".
       iModIntro.
       iSimpl.
@@ -489,32 +535,20 @@ Section copy_word.
       iApply parwp_finish.
       iApply "HΦ".
       iFrame.
-      assert (Htemp : (I0 ^+ 1)%f = step).
+      assert ((I0 ^+ 1)%f = step) as ->.
       rewrite /I0.
       simpl.
       solve_finz.
-      rewrite Htemp. clear Htemp.
-      iFrame.
-      iDestruct (big_sepL2_app_inv with "Uold") as "(Hpre & Hprog)".
-      simpl.
-      by left.
-      iFrame.
-      rewrite /c_pre.
-      iSimpl.
-      iDestruct "Hpre" as "(Hinstr1 & Hinstr2 & Hinstr3 & _)".
       iFrame.
       iSplitR "Hnz";
         last (iExists W1; iFrame).
-      assert (Htemp : ((((((progpage ^+ 3) ^+ length (prog step)) ^+ 1) ^+ 1) ^+ 1) ^+ 1)%f =
-                      (progpage ^+ S (S (S (length (prog step ++ c_post)))))%f).
+      assert ((((((progaddr ^+ length prog) ^+ 1) ^+ 1) ^+ 1) ^+ 1)%f =
+                      (progaddr ^+ (length (prog ++ c_post)))%f) as ->.
       admit.
-      rewrite Htemp. clear Htemp.
       iFrame.
-    - rename Hn into eq.
-      rename Hseq into c.
+    -
       pose proof c as Hseq.
-      apply seq_in_page_forall in c. 
-      assert (Htemp : S n = Z.to_nat (step ^- 1)%f).
+      assert (Hstep : S n = Z.to_nat (step ^- 1)%f).
       solve_finz.
       assert (Htemp' : exists (im : Imm), (step ^- 1)%f = im).
       destruct step.
@@ -526,43 +560,211 @@ Section copy_word.
         admit.
       }
       destruct Htemp' as [im Himeq].
-      rewrite Himeq in Htemp.
-      iIntros (Φ').
-      iModIntro.
-      iIntros "(HPstep & Hpc & [% Hr5] & [% Hr6] & [% Hr7] & [% Hr8] &[% Hnz] & Hacc & Hprog) HΦ".
-      rewrite <-parwp_sswp.
-      iDestruct "Hprog" as "(p_start & Hprog)". 
-      iDestruct ((mov_word (of_pid progpage) step R5) with "[Hpc Hacc Hr5 p_start]") as "J".
-      3 : { rewrite ->Forall_forall in c. apply c. set_solver. }
-      3 : { apply Hprpain. }
-      3 : { iFrame. }
-      auto.
-      by rewrite decode_encode_instruction.
+      rewrite Himeq in Hstep.
+
+      iDestruct ("Htriple" $! (S n) im _ with "") as "#HprogSpec".
+      iSpecialize ("HprogSpec"   with "[] [] ").
+      iPureIntro;lia.
+      Unshelve.
+      { admit.  }
+        assert (Htemp : (finz.seq progaddr (length prog)  ++ finz.seq (progaddr ^+ (length prog))%f 4) = finz.seq progaddr (length (prog ++ c_post))).
+        { rewrite app_length.
+          assert (length c_post = 4) as ->.
+          done.
+          rewrite (finz_seq_decomposition ((length prog) + 4) progaddr (length prog)).
+          rewrite minus_plus.
+          reflexivity.
+          lia.
+        }
+        rewrite /program' /c_loop .
+        rewrite -Htemp.
+        iDestruct (big_sepL2_app_inv with "Hprog") as "(Hprog & Hcpost)".
+        { rewrite finz_seq_length.  left;done. }
+      iDestruct ("HprogSpec" with "[HPstep Hpc Hr5 Hr6 Hr7 Hr8 Hnz Hacc Hprog ]") as "J".
+      iFrame.
+      assert (of_imm step = (im ^+ 1)%f) as ->.
+      { rewrite -Himeq.
+        solve_finz.
+        }
+      iFrame.
+      2: {  assumption. }
+      iApply parwp_parwp.
+      iApply (parwp_strong_mono with "[J]").
+      instantiate (1 := ⊤).
+      set_solver.
+      instantiate (2:=
+      (fun k => (⌜k = ExecI⌝
+                                     ∗ P im
+                                            ∗ PC @@ i ->r (progaddr ^+ (length prog))%f
+                                            ∗ R5 @@ i ->r ((of_imm im) ^+ 1)%f
+                                            ∗ R6 @@ i ->r I0
+                                            ∗ R7 @@ i ->r progaddr
+                                            ∗ (∃ r : handle, R8 @@ i ->r r)
+                                            ∗ (∃ nz, NZ @@ i ->r nz)
+                                            ∗ A@i:={q}[sacc]
+                                            ∗ program' prog  progaddr )%I)
+      ).
+      instantiate (1 := (fun k => ( ⌜k = ExecI⌝ ∗ P im ∗ PC @@ i ->r (progaddr ^+ length prog)%f ∗
+           R5 @@ i ->r (im ^+ 1)%f ∗ R6 @@ i ->r I0 ∗ R7 @@ i ->r progaddr ∗
+           (∃ r : handle, R8 @@ i ->r r) ∗ (∃ nz : handle, NZ @@ i ->r nz) ∗ A@i:={q}[sacc]  ∗
+           program' prog progaddr))%I).
       iApply "J".
       iModIntro.
-      iIntros "(Hpc & Hinstr1 & Hacc & Hr5)".
-      rewrite <-parwp_sswp.
-      iDestruct "Hprog" as "(p_start & Hprog)".
-      iDestruct ((mov_word (of_pid progpage ^+ 1)%f I0 R6) with "[Hpc Hacc Hr6 p_start]") as "J".
-      3 : { rewrite ->Forall_forall in c. apply c. set_solver. }
+      iIntros "(? & ? & ? & ? & ? & ? & ? & ? & ?)".
+      iFrame.
+      done.
+      iIntros (k) "(%Heq & HP & Hpc & Hr5 & Hr6 & Hr7 & [%r8' Hr8] & [%nz' Hnz] & Hacc & Hprog)".
+      subst k.
+      iModIntro.
+      apply seq_in_page_forall in c.
+      iDestruct "Hcpost" as "(p_start & Hcpost)".
+      iDestruct ((mov_word (progaddr ^+ length prog )%f I1 R8) with "[Hpc Hacc Hr8 p_start]") as "J".
+      5: { iFrame. }
+      3 : { instantiate (1:= progpage). rewrite ->Forall_forall in c. apply c. rewrite /c_loop. rewrite elem_of_list_In.
+            rewrite -Htemp.
+            apply in_or_app.
+            right.
+            rewrite <-elem_of_list_In.
+            set_solver.
+      }
       3 : { apply Hprpain. }
-      3 : { iFrame. }
       auto.
       by rewrite decode_encode_instruction.
+      instantiate (1 := (fun m' => (PARWP m' @ i {{ v, Φ v }})%I )).
+      instantiate (1 := ⊤).
+      iApply parwp_sswp.
       iApply "J".
       iModIntro.
-      iIntros "(Hpc & Hinstr2 & Hacc & Hr6)".
-      rewrite <-parwp_sswp.
-      iDestruct "Hprog" as "(p_start & Hprog)".
-      iDestruct ((mov_word ((of_pid progpage ^+ 1) ^+ 1)%f base R7) with "[Hpc Hacc Hr7 p_start]") as "J".
-      3 : { rewrite ->Forall_forall in c. apply c. set_solver. }
+      iIntros "(Hpc & Hinstr4 & Hacc & Hr8)".
+      iApply parwp_sswp.
+      iDestruct "Hcpost" as "(p_start & Hcpost)".
+      iDestruct ((sub ((progaddr ^+ length prog ) ^+ 1)%f R5 R8) with "[Hpc Hacc Hr5 Hr8 p_start]") as "J".
+      5: { iFrame. }
+      3 : { instantiate (1:= progpage). rewrite ->Forall_forall in c. apply c. rewrite /c_loop. rewrite elem_of_list_In.
+            rewrite -Htemp.
+            apply in_or_app.
+            right.
+            rewrite <-elem_of_list_In.
+            set_solver.
+      }
       3 : { apply Hprpain. }
-      3 : { iFrame. }
       auto.
       by rewrite decode_encode_instruction.
+      instantiate (1 := (fun m' => (PARWP m' @ i {{ v, Φ v }})%I )).
       iApply "J".
       iModIntro.
-      iIntros "(Hpc & Hinstr3 & Hacc & Hr7)".
+      iIntros "(Hpc & Hinstr5 & Hr5 & Hr8 & Hacc)".
+      iApply parwp_sswp.
+      iDestruct "Hcpost" as "(p_start & Hcpost)".
+      iDestruct ((cmp_reg (((progaddr ^+ length prog ) ^+ 1) ^+ 1)%f R6 R5) with "[Hpc Hacc Hr5 Hr6 Hnz p_start]") as "J".
+      5: {iFrame. }
+      3 : { instantiate (1:= progpage). rewrite ->Forall_forall in c. apply c. rewrite /c_loop. rewrite elem_of_list_In.
+            rewrite -Htemp.
+            apply in_or_app.
+            right.
+            rewrite <-elem_of_list_In.
+            set_solver.
+      }
+      reflexivity.
+      apply decode_encode_instruction.
+      apply Hprpain.
+      iFrame.
+      instantiate (1 := (fun m' => (PARWP m' @ i {{ v, Φ v }})%I )).
+      iApply "J".
+      iModIntro.
+      iIntros "(Hpc & Hinstr6 & Hr6 & Hr5 & Hacc & Hnz)".
+      assert ((I0 <? im ^+ 1 ^- I1)%f = true) as ->.
+      {
+        rewrite /I0 /I1 -Himeq /= .
+        solve_finz.
+      }
+      iApply parwp_sswp.
+      iDestruct "Hcpost" as "(p_start & Hcpost)".
+      iDestruct ((bne ((((progaddr ^+ length prog ) ^+ 1) ^+ 1) ^+ 1)%f R7) with "[Hpc Hacc Hr7 Hnz p_start]") as "J".
+      5 : { iFrame. }
+      3 : { instantiate (1:= progpage). rewrite ->Forall_forall in c. apply c. rewrite /c_loop. rewrite elem_of_list_In.
+            rewrite -Htemp.
+            apply in_or_app.
+            right.
+            rewrite <-elem_of_list_In.
+            set_solver.
+      }
+      reflexivity.
+      apply decode_encode_instruction.
+      apply Hprpain.
+      instantiate (1 := (fun m' => (PARWP m' @ i {{ v, Φ v }})%I )).
+      iApply "J".
+      iModIntro.
+      iSimpl.
+      iIntros "(Hpc & Hinstr7 & Hr7 & Hacc & Hnz)".
+      assert ((im ^+ 1 ^- I1)%f = im) as ->.
+      {
+        rewrite /I1 /=.
+        solve_finz.
+      }
+      iApply ("IH" $! im with "[] [] [] HP Hpc Hr5 Hr6 Hr7 [Hr8] [Hnz] Hacc [Hprog Hinstr4 Hinstr5 Hinstr6 Hinstr7]  [HΦ]").
+      {
+      iPureIntro.
+      rewrite -Himeq.
+        solve_finz.
+      }
+      {
+        done.
+      }
+      iModIntro.
+      iIntros (v_ v'_ ) "%Hv_ %Hv'_".
+      iApply ("Htriple" $! v_ v'_ ).
+      { iPureIntro.
+        lia.
+      }
+      { iPureIntro.
+        lia.
+      }
+      iExists I1;iFrame.
+      iExists W2;iFrame.
+      iFrame.
+      done.
+      assert ((step ^- S (S n))%f = (im ^- S n)%f) as ->.
+      solve_finz.
+      iFrame.
+
+
+      (* iIntros (Φ'). *)
+      (* iModIntro. *)
+      (* iIntros "(HPstep & Hpc & [% Hr5] & [% Hr6] & [% Hr7] & [% Hr8] &[% Hnz] & Hacc & Hprog) HΦ". *)
+      (* rewrite <-parwp_sswp. *)
+      (* iDestruct "Hprog" as "(p_start & Hprog)".  *)
+      (* iDestruct ((mov_word (of_pid progpage) step R5) with "[Hpc Hacc Hr5 p_start]") as "J". *)
+      (* 3 : { rewrite ->Forall_forall in c. apply c. set_solver. } *)
+      (* 3 : { apply Hprpain. } *)
+      (* 3 : { iFrame. } *)
+      (* auto. *)
+      (* by rewrite decode_encode_instruction. *)
+      (* iApply "J". *)
+      (* iModIntro. *)
+      (* iIntros "(Hpc & Hinstr1 & Hacc & Hr5)". *)
+      (* rewrite <-parwp_sswp. *)
+      (* iDestruct "Hprog" as "(p_start & Hprog)". *)
+      (* iDestruct ((mov_word (of_pid progpage ^+ 1)%f I0 R6) with "[Hpc Hacc Hr6 p_start]") as "J". *)
+      (* 3 : { rewrite ->Forall_forall in c. apply c. set_solver. } *)
+      (* 3 : { apply Hprpain. } *)
+      (* 3 : { iFrame. } *)
+      (* auto. *)
+      (* by rewrite decode_encode_instruction. *)
+      (* iApply "J". *)
+      (* iModIntro. *)
+      (* iIntros "(Hpc & Hinstr2 & Hacc & Hr6)". *)
+      (* rewrite <-parwp_sswp. *)
+      (* iDestruct "Hprog" as "(p_start & Hprog)". *)
+      (* iDestruct ((mov_word ((of_pid progpage ^+ 1) ^+ 1)%f base R7) with "[Hpc Hacc Hr7 p_start]") as "J". *)
+      (* 3 : { rewrite ->Forall_forall in c. apply c. set_solver. } *)
+      (* 3 : { apply Hprpain. } *)
+      (* 3 : { iFrame. } *)
+      (* auto. *)
+      (* by rewrite decode_encode_instruction. *)
+      (* iApply "J". *)
+      (* iModIntro. *)
+      (* iIntros "(Hpc & Hinstr3 & Hacc & Hr7)". *)
       iDestruct ("Htriple" $! (S n) im I0 step _ with "") as "#HprogSpec".
       Unshelve.
       2 : {
@@ -590,11 +792,6 @@ Section copy_word.
       admit.
       rewrite Hn.
       clear Hn.
-      iFrame.
-      iSplitL "Hr8".
-      iExists r8.
-      iFrame.
-      iExists nz.
       iFrame.
       iApply parwp_parwp.
       iApply (parwp_strong_mono with "[J]").
@@ -762,7 +959,8 @@ Section copy_word.
       iModIntro.
       iSimpl.
       iIntros "(Hpc & Hinstr7 & Hr7 & Hacc & Hnz)".
-      iApply ("IH" $! im with "[] [] [] [] [HP Hpc Hr5 Hr6 Hr7 Hr8 Hnz Hacc Uold Hinstr4 Hinstr5 Hinstr6 Hinstr7]").
+      iDestruct "Uold" as  "(Hinstr1 & Hinstr2 & Hinstr3 & Uold)".
+      iApply ("IH" $! im with "[] [] [] [] HP [Hr8] [Hnz] [Hinstr4 Hinstr5 Hinstr6 Hinstr7]  [HΦ] Hinstr1 Hr5 Hinstr5 Hinstr6 Hr6 Hpc Hinstr7 Hacc Hr7").
       {
       iPureIntro.
       rewrite -Himeq.
